theories/rule_misc.v
@@ -541,21 +541,21 @@ From HypVeri Require Import RAs.
   Qed.
 
 
-  Lemma update_current_vmid_preserve_receivers σ i : get_receivers_gmap (update_current_vmid σ i) =
-                                               (get_receivers_gmap σ).
+  Lemma update_current_vmid_preserve_receivers σ i : get_retrieved_gmap (update_current_vmid σ i) =
+                                               (get_retrieved_gmap σ).
   Proof.
-    rewrite /get_receivers_gmap.
+    rewrite /get_retrieved_gmap.
     f_equal.
   Qed.
 
-  Lemma update_reg_global_preserve_receivers σ i r w : get_receivers_gmap (update_reg_global σ i r w) =
-                                               (get_receivers_gmap σ).
+  Lemma update_reg_global_preserve_receivers σ i r w : get_retrieved_gmap (update_reg_global σ i r w) =
+                                               (get_retrieved_gmap σ).
   Proof.
-    rewrite /get_receivers_gmap.
+    rewrite /get_retrieved_gmap.
     f_equal.
   Qed.
 
-  Lemma update_offset_PC_preserve_receivers σ o : get_receivers_gmap (update_offset_PC σ o) = get_receivers_gmap σ.
+  Lemma update_offset_PC_preserve_receivers σ o : get_retrieved_gmap (update_offset_PC σ o) = get_retrieved_gmap σ.
   Proof.
     unfold update_offset_PC.
     destruct (get_vm_reg_file σ (get_current_vm σ) !! PC).
@@ -563,10 +563,10 @@ From HypVeri Require Import RAs.
     done.
   Qed.
 
- Lemma update_memory_unsafe_preserve_receivers σ a w : get_receivers_gmap (update_memory_unsafe σ a w) =
-                                               (get_receivers_gmap σ).
+ Lemma update_memory_unsafe_preserve_receivers σ a w : get_retrieved_gmap (update_memory_unsafe σ a w) =
+                                               (get_retrieved_gmap σ).
   Proof.
-    rewrite /get_receivers_gmap.
+    rewrite /get_retrieved_gmap.
     f_equal.
   Qed.
 
@@ -651,9 +651,9 @@ Qed.
       f_equal.
 Qed.
    Lemma update_ownership_batch_preserve_receivers σ (ps: list PID) perm:
-   get_receivers_gmap (update_ownership_batch σ ps perm) = get_receivers_gmap σ.
+   get_retrieved_gmap (update_ownership_batch σ ps perm) = get_retrieved_gmap σ.
     Proof.
-      rewrite /get_receivers_gmap.
+      rewrite /get_retrieved_gmap.
       f_equal.
 Qed.
 
@@ -728,9 +728,9 @@ Qed.
       f_equal.
 Qed.
    Lemma update_access_batch_preserve_receivers σ (ps: list PID) perm:
-   get_receivers_gmap (update_access_batch σ ps perm) = get_receivers_gmap σ.
+   get_retrieved_gmap (update_access_batch σ ps perm) = get_retrieved_gmap σ.
     Proof.
-      rewrite /get_receivers_gmap.
+      rewrite /get_retrieved_gmap.
       f_equal.
 Qed.
 
@@ -827,7 +827,7 @@ Qed.
             done.
         Qed.
 
-    Lemma update_access_batch_noaccess{ σ i sacc} {sps:gset PID} (ps: list PID):
+    Lemma update_access_batch_update_access_noaccess{ σ i sacc} {sps:gset PID} (ps: list PID):
      sps = (list_to_set ps)->
      i = (get_current_vm σ) ->
      (get_access_gmap σ) !! i = Some (DfracOwn 1, to_agree (GSet sacc)) ->
@@ -1069,7 +1069,7 @@ Qed.
         Qed.
 
 
-    Lemma update_page_table_batch_update_own_owned{ σ i sown} {sps:gset PID} (ps: list PID):
+    Lemma update_ownership_batch_update_own_owned{ σ i sown} {sps:gset PID} (ps: list PID):
      sps = (list_to_set ps)->
      i = (get_current_vm σ) ->
      (get_owned_gmap σ) !! i = Some (DfracOwn 1, to_agree (GSet sown)) ->
@@ -1302,6 +1302,250 @@ Qed.
             by subst.
       Qed.
 
+            Lemma get_excl_gmap_is_exclusive_true {σ i sexcl} p:
+            (get_excl_gmap σ) !! i = Some (DfracOwn 1, to_agree (GSet sexcl))->
+            (p ∈ sexcl<->
+            ∃ perm, (get_vm_page_table σ i).2 !! p =Some perm ∧ is_exclusive perm = true).
+        Proof.
+          intros.
+          rewrite /get_excl_gmap in H.
+          apply (elem_of_list_to_map_2 _ i (DfracOwn 1, to_agree (GSet sexcl))) in H.
+          inv_map_in. clear H0.
+          inversion H.
+          subst.
+          clear H.
+          split.
+          - intro H. apply elem_of_list_to_set in H.
+            inv_map_in.
+          apply elem_of_list_In in H0.
+          apply elem_of_map_to_list' in H0.
+          apply map_filter_lookup_Some in H0.
+          destruct H0.
+          exists x.2.
+          split;eauto.
+          by subst p.
+          - intros H.
+            destruct H.
+            apply elem_of_list_to_set.
+            apply elem_of_list_In.
+            apply in_map_iff.
+            exists (p,x).
+            split;eauto.
+            apply elem_of_list_In.
+            apply elem_of_map_to_list'.
+            apply map_filter_lookup_Some.
+            done.
+        Qed.
+
+
+  Lemma update_access_batch_update_excl_noaccess{ σ i sexcl} {sps:gset PID} (ps: list PID):
+     sps = (list_to_set ps)->
+     i = (get_current_vm σ) ->
+     (get_excl_gmap σ) !! i = Some (DfracOwn 1, to_agree (GSet sexcl)) ->
+     get_excl_gmap (update_access_batch σ ps NoAccess) =
+     <[(get_current_vm σ):= (DfracOwn 1, to_agree (GSet (sexcl ∖ sps ) ))]>(get_excl_gmap σ).
+         Proof.
+        intros.
+        rewrite /get_excl_gmap.
+        apply (@map_eq VMID (gmap VMID) _ _ _ _ _ _ _ _ gmap_finmap);eauto.
+        intro.
+        rewrite -H0.
+        destruct(decide (i0 = i)).
+        - subst i0. rewrite lookup_insert.
+          apply (@elem_of_list_to_map_1' VMID (gmap VMID) _ _ _ _ _ _ _ _ gmap_finmap).
+          + intros.
+            inv_map_in.
+             inversion H2.
+             do 3 f_equal.
+             clear H6 H3 H2.
+             subst x.
+             symmetry.
+             apply set_eq.
+             intro.
+             rewrite  elem_of_list_to_set.
+             split.
+            * intros.
+              inv_map_in.
+              apply elem_of_list_In in H3.
+              apply (elem_of_map_to_list' _ x0) in H3.
+              apply map_filter_lookup_Some in H3.
+              destruct H3.
+              simplify_eq /=.
+              rewrite /get_vm_page_table /get_page_tables /update_access_batch
+                      /update_access_global_batch //= in H3.
+              rewrite vlookup_insert in H3.
+              apply elem_of_difference.
+              induction ps; simpl in *.
+              -- split;[|set_solver].
+                 apply (get_excl_gmap_is_exclusive_true x0.1 H1).
+                 exists (x0.2).
+                 split;eauto.
+              -- assert (Hneq: a ≠ x0.1).
+                 { destruct (decide (a=x0.1));eauto.
+                   subst a.
+                   rewrite lookup_insert in H3.
+                   inversion H3.
+                   rewrite -H0 in H4.
+                   rewrite /is_exclusive // in H4.
+                 }
+                 rewrite not_elem_of_union.
+                 assert (Himp : x0.1 ∈ sexcl ∧ x0.1 ∉ ((list_to_set ps):gset PID)
+                  ->(x0.1 ∈ sexcl ∧ (x0.1 ∉ ({[a]}:gset PID)) ∧ x0.1 ∉ ((list_to_set ps):gset PID))).
+                 { intros. destruct H; split;eauto. split. set_solver. done. }
+                 apply Himp.
+                 apply IHps;eauto.
+                 rewrite lookup_insert_ne in H3;done.
+            * intros.
+              apply elem_of_difference in H2.
+              destruct H2.
+              apply (get_excl_gmap_is_exclusive_true x H1) in H2;eauto.
+              destruct H2.
+              destruct H2.
+              inv_map_in.
+              exists (x,x0).
+              split;eauto.
+              apply elem_of_list_In .
+              apply  elem_of_map_to_list.
+              apply map_filter_lookup_Some.
+              rewrite /get_vm_page_table /get_page_tables /update_access_batch
+                      /update_access_global_batch /=.
+              rewrite -H0 vlookup_insert.
+              destruct H1;split;eauto.
+              generalize dependent sps.
+              induction ps;simpl.
+              done.
+              intros.
+              rewrite H //= in H3.
+              assert (Hneq: a ≠ x).
+              { set_solver. }
+              rewrite lookup_insert_ne;eauto.
+              apply (IHps (list_to_set ps));eauto.
+              set_solver.
+          + inv_map_in.
+            exists i.
+            split;[|apply in_list_of_vmids].
+            do 4 f_equal.
+            apply set_eq.
+            intro.
+            rewrite  elem_of_list_to_set.
+            split.
+            -- intros.
+               inv_map_in.
+               subst x.
+               apply elem_of_list_In in H3.
+               apply (elem_of_map_to_list' _ x0) in H3.
+               apply map_filter_lookup_Some in H3.
+               destruct H3.
+               rewrite /get_vm_page_table /get_page_tables /update_access_batch
+                       /update_access_global_batch //= in H2.
+               rewrite -H0 vlookup_insert in H2.
+               apply elem_of_difference.
+               generalize dependent sps.
+               induction ps; simpl in *.
+               ++ intros.
+                 split;[|set_solver].
+                 apply (get_excl_gmap_is_exclusive_true x0.1 H1).
+                 exists x0.2.
+                 split;eauto.
+               ++ intros.
+                 assert (Hneq: a ≠ x0.1).
+                 { destruct (decide (a=x0.1));eauto.
+                   subst a.
+                   rewrite lookup_insert in H2.
+                   inversion H2.
+                   rewrite -H5 in H3.
+                   done.
+                 }
+                 rewrite H.
+                 rewrite not_elem_of_union.
+                 assert (Himp : x0.1 ∈ sexcl ∧ x0.1 ∉ ((list_to_set ps):gset PID)
+                  ->(x0.1 ∈ sexcl ∧ (x0.1 ∉ ({[a]}:gset PID)) ∧ x0.1 ∉ ((list_to_set ps):gset PID))).
+                 {  intros. destruct H4; split;eauto. split. set_solver. done. }
+                 apply Himp.
+                 apply IHps;eauto.
+                 rewrite lookup_insert_ne //= in H2.
+            -- intros.
+               apply elem_of_difference in H2.
+               destruct H2.
+               apply (get_excl_gmap_is_exclusive_true x H1) in H2;eauto.
+               destruct H2.
+               destruct H2.
+               inv_map_in.
+               exists (x,x0).
+               split;eauto.
+                 apply elem_of_list_In .
+                 apply  elem_of_map_to_list.
+                 apply map_filter_lookup_Some.
+                 rewrite /get_vm_page_table /get_page_tables /update_access_batch
+                         /update_access_global_batch /=.
+                 rewrite -H0 vlookup_insert.
+                 destruct H1;split;eauto.
+                 generalize dependent sps.
+                 induction ps;simpl.
+                 done.
+                 intros.
+                 rewrite H in H3.
+                 simpl in H3.
+                 assert (Hneq: a ≠ x).
+                 { set_solver. }
+                 rewrite lookup_insert_ne;eauto.
+                 apply (IHps (list_to_set ps));eauto.
+                 set_solver.
+        - rewrite (lookup_insert_ne _ i i0 _);eauto.
+          set (l:= (map
+              (λ v : VMID,
+              (v, (DfracOwn 1,
+                   to_agree (GSet
+                               (list_to_set
+                                  (map (λ p : PID * access, p.1)
+                      (map_to_list
+            (filter (λ p : PID * access, is_exclusive p.2 = true) (get_vm_page_table σ v).2))))))))
+                      list_of_vmids)) in *.
+          destruct (list_to_map l !! i0) eqn:Heqn.
+          + apply (elem_of_list_to_map_2 l i0 c) in Heqn.
+            apply elem_of_list_In in Heqn.
+            apply in_map_iff in Heqn.
+            inversion Heqn;clear Heqn.
+            destruct H2 as [H3 HIn];inversion H3;subst;clear H3.
+            apply (@elem_of_list_to_map_1' VMID (gmap VMID) _ _ _ _ _ _ _ _ gmap_finmap).
+            *  intros.
+               inv_map_in.
+               inversion H.
+               do 7 f_equal.
+               rewrite /get_vm_page_table update_access_batch_preserve_other_page_tables //.
+            * inv_map_in.
+              exists i0.
+              split;eauto.
+              do 8 f_equal.
+              rewrite /get_vm_page_table update_access_batch_preserve_other_page_tables //.
+          + apply (@not_elem_of_list_to_map_2 VMID (gmap VMID) _ _ _ _ _ _ _ _ gmap_finmap) in Heqn.
+            apply (@not_elem_of_list_to_map_1 VMID (gmap VMID) _ _ _ _ _ _ _ _ gmap_finmap).
+            intro P.
+            apply Heqn.
+            apply elem_of_list_In.
+            apply in_map_iff.
+            apply elem_of_list_In in P.
+            apply in_map_iff in P.
+            destruct P.
+            exists x.
+            destruct H2.
+            split;eauto.
+            apply in_map_iff.
+            apply in_map_iff in H3.
+            destruct H3.
+            exists x0.
+            destruct H3.
+            split;eauto.
+            rewrite -H3.
+            do 8 f_equal.
+            rewrite /get_vm_page_table update_access_batch_preserve_other_page_tables //.
+            destruct x.
+            simpl in H2;inversion H3.
+            by subst.
+      Qed.
+
+
+
   Lemma insert_transaction_preserve_current_vm σ h trans:
    get_current_vm (insert_transaction σ h trans) = get_current_vm σ.
     Proof.
@@ -1363,8 +1607,21 @@ Qed.
       rewrite /get_excl_gmap.
       f_equal.
 Qed.
+    (*TODO *)
+    Lemma insert_transaction_update_trans σ h tran:
+     (get_trans_gmap (insert_transaction σ h tran)) = <[h:=tran]>(get_trans_gmap σ).
+      Proof.
+      Admitted.
 
+    Lemma insert_transaction_update_hpool σ h tran:
+     (get_hpool_gset (insert_transaction σ h tran)) = (get_hpool_gset σ) ∖ {[h]}.
+      Proof.
+        Admitted.
 
+    Lemma insert_transaction_update_trans σ h tran:
+     (get_retrieved_gmap (insert_transaction σ h tran)) = <[h:=false]>(get_retrieved_gmap σ).
+      Proof.
+        Admitted.
 
  (* TODO more preserving rules. *)
 
